src/Specifications.v
@@ -1,0 +1,147 @@
+Require Import AsyncDisk.
+Require Import MemClass Pred PredCrash.
+Require Import Prog ProgMonad Hoare.
+Require Import SepAuto.
+Require Import Hashmap.
+
+Set Implicit Arguments.
+
+Notation prog_valuset := (valu * list valu)%type.
+
+Record SeqHoareSpec R :=
+  SeqSpec { seq_spec_pre: @pred addr _ prog_valuset;
+            seq_spec_post: R -> @pred addr _ prog_valuset;
+            seq_spec_crash: @pred addr _ prog_valuset }.
+
+Definition seq_hoare_double R A (spec: A -> SeqHoareSpec R)
+           (p: Prog.prog R) :=
+  forall T' (rx : R -> Prog.prog T'),
+    Hoare.corr2
+      (fun hm_ done_ crash_ =>
+         exists a F_,
+           F_ * seq_spec_pre (spec a) *
+           [[ sync_invariant F_ ]] *
+           [[ forall r, Hoare.corr2
+                       (fun hm'_ done'_ crash'_ =>
+                          F_ * seq_spec_post (spec a) r  *
+                          [[ exists l, hashmap_subset l hm_ hm'_ ]] *
+                          [[ done'_ = done_ ]] *
+                          [[ crash'_ = crash_ ]]
+                       ) (rx r) ]] *
+           [[ forall hm_crash,
+                (F_ * seq_spec_crash (spec a) *
+                 [[ exists l, hashmap_subset l hm_ hm_crash ]])%pred =p=>
+              crash_ hm_crash ]])%pred
+      (Bind p rx).
+
+Section ExampleSeqSpecs.
+
+  (* isomorphic to prod, but distinct for the benefit of Ltac *)
+  Inductive spec_prod A B :=
+    spec_pair : A -> B -> spec_prod A B.
+
+  Ltac destruct_spec_prod :=
+    repeat match goal with
+    | [ p: spec_prod _ _ |- _ ] => destruct p
+    end.
+
+  Ltac spec_equiv :=
+    repeat lazymatch goal with
+           | [ |- forall _, _ ] => intros
+           | [ |- seq_hoare_double _ _ ] =>
+             unfold seq_hoare_double
+           | [ |- corr2 _ _ ] =>
+             eapply pimpl_ok2; [ solve [ eauto ] | eauto ]
+           | [ |- _ =p=> exists (_: spec_prod _ _), _ ] =>
+             eapply pimpl_exists_l;
+             intros;
+             repeat destruct_spec_prod;
+             cancel
+           | [ |- _ =p=> _ ] =>
+             cancel
+           end.
+
+  (* these are the sorts of theorems needed to go from the notation to
+  the more structured SeqHoareSpec. *)
+  Theorem seq_read_spec : forall a,
+      {< v,
+       PRE        a |-> v
+       POST RET:r a |-> v * [[ r = (fst v) ]]
+       CRASH      a |-> v
+      >} Prog.Read a <->
+      seq_hoare_double
+        (fun v =>
+           SeqSpec (a |-> v)%pred
+                   (fun r => a |-> v *
+                                 [[ r = (fst v) ]])%pred
+                   (a |-> v)%pred
+        ) (Prog.Read a).
+  Proof.
+    split; intros.
+    - spec_equiv.
+    - spec_equiv.
+  Qed.
+
+  Definition swap a a' :=
+    v <- Prog.Read a;
+      v' <- Prog.Read a';
+      Prog.Write a v';;
+      Prog.Write a' v;;
+      Ret tt.
+
+  Notation "'SEQSPEC' e1 .. e2 , {{ pre }} {{ post }} {{ crash }}" :=
+    (fun e1 => .. (fun e2 =>
+                  SeqSpec pre%pred post%pred crash%pred) .. )
+      (at level 0,
+       e1 binder,
+       e2 binder).
+
+  Definition uncurry {A B C} (f: A -> B -> C) :
+    spec_prod A B -> C :=
+    fun ab => let 'spec_pair a b := ab in f a b.
+
+  Definition test_spec a a' :=
+    uncurry SEQSPEC v v',
+    {{ a |-> v * a' |-> v' }}
+      {{ fun r:unit => a |-> v' * a' |-> v }}
+      {{ a |->? * a' |->? }}.
+
+  Hint Resolve spec_pair.
+
+  Theorem seq_swap_spec : forall a a',
+      {< (v v': prog_valuset),
+       PRE       a |-> v * a' |-> v'
+       POST RET:_ a |-> v' * a' |-> v
+       CRASH a |->? * a' |->?
+      >} swap a a' <->
+      seq_hoare_double
+        (uncurry SEQSPEC v v',
+         {{ a |-> v * a' |-> v' }}
+           {{ fun r:unit => a |-> v' * a' |-> v }}
+           {{ a |->? * a' |->? }}
+        ) (swap a a').
+  Proof.
+    unfold uncurry.
+    split; intros.
+
+    - (* this is exactly what spec_equiv does, but cancel exposes a bug
+    that prevents the tactic from working *)
+      unfold seq_hoare_double; intros.
+      eapply pimpl_ok2; eauto; intros.
+      eapply pimpl_exists_l.
+      intros.
+      destruct_spec_prod.
+      cancel.
+
+    - eapply pimpl_ok2; eauto; intros.
+      (* this looks bad, but its just deex'ing the number of
+      existentially quantified variables in the precondition, then
+      instantiating the pair on the right hand side with the newly
+      created sequence of variables *)
+      do 2 (eapply pimpl_exists_l; intros; eauto).
+      apply pimpl_exists_r.
+      exists (spec_pair x x0).
+      cancel.
+  Qed.
+
+End ExampleSeqSpecs.
